## SUSTech DSP tutorial 11

#### 12110623 曹正阳

## Q1 
**Type I:** The impulse response is symmetric and N an odd integer 

When $N_1 = 2, N_2 = 0, N_3 = 0, N_4 = 0$; $H(z) = (1 + z^{-1})^2 = 1 + 2 z^{-1} + z^{-2}$
When $N_1 = 0, N_2 = 2, N_3 = 0, N_4 = 0$; $H(z) = (1 - z^{-1})^2 = 1 - 2 z^{-1} + z^{-2}$
When $N_1 = 0, N_2 = 0, N_3 = 1, N_4 = 0$; $H(z) = 1 + \alpha_i z^{-1} + z^{-2}$


**Type II:** The impulse response is symmetric and N an even integer 

When $N_1 = 1, N_2 = 0, N_3 = 0, N_4 = 0$; $H(z) = 1 + z^{-1}$


**Type III:** The impulse response is anti-symmetric and N an odd integer 

When $N_1 = 1, N_2 = 1, N_3 = 0, N_4 = 0$; $H(z) = (1 + z^{-1}) (1 - z^{-1}) = 1 + 0z^{-1}- z^{-2}$


**Type IV:** The impulse response is anti-symmetric and N an even integer 

When $N_1 = 0, N_2 = 1, N_3 = 0, N_4 = 0$; $H(z) = 1 - z^{-1}$


## Q2

$\alpha = \frac{1-sin(\omega_c)}{cos(\omega_c)} = \frac{1-sin(0.42)}{cos(0.42)} = 0.648611018$

So $H(z) = \frac{1+\alpha}{2} \frac{1—z^{-1}}{1—\alpha z^{-1}} =\frac{0.1757(1 + z^{-1})}{1 - 0.6486z^{-1}}$

## Q3

#### (a)

$|H_{BS}(z)|^2 = |H_{BS}(e^{j\omega})*H_{BS}(e^{-j\omega})|$

$|H_{BS}(z)|^2 = (\frac{1+\alpha}{2})^2*(\frac{1-2\beta z^{-1} + z^{-2}}{1-\beta (1+\alpha)z^{-1} + \alpha z^{-2}})^2  = (\frac{1+\alpha}{2})^2 * \frac{1- 4 \beta z^{-1} +(4 \beta^{2}+2) z^{-2} - 4 \beta z^{-3}  + z^{-4}}{    \alpha^{2}- (2 \alpha^{2} \beta - 2 \alpha \beta)z^{-1} + (\alpha^{2} \beta^{2}+ 2 \alpha \beta^{2} + 2 \alpha + \beta^{2})z^{-2}   - (2 \alpha \beta + 2 \beta) z^{-3} + z^{-4}}
$

#### (b)
$|H_{BS}(e^{j\omega})|^2 = \left(\frac{1+\alpha}{2}\right)^2 \cdot \frac{1 - 4\beta e^{-j\omega} + (4\beta^2 + 2)e^{-2j\omega} - 4\beta e^{-3j\omega} + e^{-4j\omega}}{\alpha^2 - (2\alpha^2\beta - 2\alpha\beta)e^{-j\omega} + (\alpha^2\beta^2 + 2\alpha\beta^2 + 2\alpha + \beta^2)e^{-2j\omega} - (2\alpha\beta + 2\beta)e^{-3j\omega} + e^{-4j\omega}} = \left(\frac{1+\alpha}{2}\right)^2 \cdot\frac{2 \cos 2 \omega - 8 \beta \cos \omega + 2 + 4 \beta^2}{2 \alpha \cos 2 \omega - 2 \beta (1+\alpha)^{2} \cos \omega + 1 + \alpha^2 + \beta^2 (1+\alpha)^{2}}$


when $\omega = cos^{-1}(\beta)$, $|H_{BS}(e^{jcos^{-1}(\beta)})|^2 = \left(\frac{1+\alpha}{2}\right)^2 \cdot\frac{2 \cos 2 cos^{-1}(\beta) - 8 \beta \cos cos^{-1}(\beta) + 2 + 4 \beta^2}{2 \alpha \cos 2 cos^{-1}(\beta) - 2 \beta (1+\alpha)^{2} \cos cos^{-1}(\beta) + 1 + \alpha^2 + \beta^2 (1+\alpha)^{2}} =\left(\frac{1+\alpha}{2}\right)^2 \cdot\frac{0}{\dots} = 0$


#### (c)

$|H_{BS}(e^{j\omega})|^2 = \left(\frac{1+\alpha}{2}\right)^2 \cdot \frac{2 \cos 2 \omega - 8 \beta \cos \omega + 2 + 4 \beta^2}{2 \alpha \cos 2 \omega - 2 \beta (1+\alpha)^{2} \cos \omega + 1 + \alpha^2 + \beta^2 (1+\alpha)^{2}}$

when $\omega = 0$, $|H_{BS}(e^{j\omega})|^2 = \left(\frac{1+\alpha}{2}\right)^2 \cdot \frac{4}{1+2\alpha+\alpha^2} = 1$

when $\omega = \pi$, $|H_{BS}(e^{j\omega})|^2 = \left(\frac{1+\alpha}{2}\right)^2 \cdot \frac{4}{1+2\alpha+\alpha^2} = 1$

#### (d)

$|H_{BS}(e^{j\omega})|^2 = \frac{1}{2} \Rightarrow B_\omega = cos^{-1}(\frac{2\alpha}{1+\alpha^2}) $


## Q4

$cos^{-1}(\beta) = 0.35\pi \Rightarrow \beta = cos(0.35\pi) = 0.4539905$


$B_w = \cos^{-1} \left( \frac{2 \alpha}{1 + \alpha^2} \right) = 0.15\pi \Rightarrow \alpha^2 +1 -\frac{1}{cos(0.15\pi)}\alpha = 0 \Rightarrow \alpha = e^{-0.31\pi}$

So $H_{BS}(z) = \frac{1+e^{-0.31\pi}}{2} * \frac{1-0.9 z^{-1} + z^{-2}}{0.55 (1+e^{-0.31\pi})z^{-1} + e^{-0.31\pi} z^{-2}}$


## Q5
$|A_M(e^{j\omega})|^2 = A_M(e^{j\omega}) \cdot A_M(e^{-j\omega}) = 1$
So, it is a allpass filter

As for causality and stability, similar to real-coefficient allpass transfer function, the root of the denominator is also within the unit circle, the poles and zeros are conjugate pairs.

## Q6

$H_1(z) = 2.5(1 - 1.6z^{-1} + 2z^{-2})(1 + 1.6z^{-1} + z^{-2})(1 + z^{-1})(1 - 0.8z^{-1} + 0.5z^{-2})$

#### (a)
the only zero outside the unit circle is come from $1 - 1.6z^{-1} + 2z^{-2}$, so substitude it with $2 - 1.6z^{-1} + 1z^{-2}$
$H_2(z) = H_1(z)\frac{2 - 1.6z^{-1} + 1z^{-2}}{1 - 1.6z^{-1} + 2z^{-2}} = 2.5(2 - 1.6z^{-1} + 1z^{-2})(1 + 1.6z^{-1} + z^{-2})(1 + z^{-1})(1 - 0.8z^{-1} + 0.5z^{-2})$

#### (b)
the only zero inside the unit circle is come from $1 - 0.8z^{-1} + 0.5z^{-2}$, so substitude it with $0.5 - 0.8z^{-1} + 1z^{-2}$
$H_3(z) = H_1(z)\frac{0.5 - 0.8z^{-1} + 1z^{-2}}{1 - 0.8z^{-1} + 0.5z^{-2}} = 2.5(1 - 1.6z^{-1} + 2z^{-2})(1 + 1.6z^{-1} + z^{-2})(1 + z^{-1})(0.5 - 0.8z^{-1} + 1z^{-2})$

#### (c)

there is no more combination of poles and zeros to satisfy the magnitude response.

## Q7

To fix the sound issues caused by the channel, we need a special filter at the receiving end. This filter, let's call it \(G(z)\), should make the overall sound transfer, \(H(z)G(z)\), have an even volume across different frequencies.

The channel's sound behavior is described by \(H(z)\), and it's a bit wonky:
\[ H(z) = \frac{(2.2 + 5z^{-1})(1 - 3.1z^{-1})}{(1 + 0.81z^{-1})(1 - 0.62z^{-1})} \]

To create \(G(z)\), we kind of do the opposite of what the channel does. So, \(G(z)\) is like the "flip side" of \(H(z)\):
\[ G(z) = \frac{(1 + 0.81z^{-1})(1 - 0.62z^{-1})}{(2.2 + 5z^{-1})(1 - 3.1z^{-1})} \]

This \(G(z)\) acts as a sort of equalizer, balancing out the sound, making everything sound more natural and clear.

## Q8
$ 0<K<0.5 $

## Q9
$C(z)=\frac{0.3+0.1167z^{-1}-0.4533z^{-2}-1.0717z^{-3}-0.9338z^{-4}-0.4819z}{z^{-1}+2.35z^{-2}+2.925z^{-3}+1.6875+0.5063z^{-5}}$